src/BinEncoders/Env/Common/Specs.v
@@ -1,7 +1,11 @@
 Require Export
         Coq.Lists.List
+        Fiat.Common
+        Fiat.Computation.Notations
         Fiat.BinEncoders.Env.Common.Transformer
         Fiat.BinEncoders.Env.Common.Cache.
+
+Delimit Scope binencoders_scope with binencoders.
 
 Set Implicit Arguments.
 
@@ -28,10 +32,39 @@ Section Specifications.
              (predicate : A -> Prop)
              (encode : A -> CacheEncode -> B * CacheEncode)
              (decode : B -> CacheDecode -> option (A * B * CacheDecode)) :=
-    forall env env' xenv xenv' data data' bin ext ext',
+    forall env env' xenv data bin ext,
       Equiv env env' ->
       predicate data ->
       encode data env = (bin, xenv) ->
-      decode (transform bin ext) env' = Some (data', ext', xenv') ->
-      Equiv xenv xenv' /\ data = data' /\ ext = ext'.
+      exists xenv',
+        decode (transform bin ext) env' = Some (data, ext, xenv')
+        /\ Equiv xenv xenv'.
+
+  Definition DecodeBindOpt2
+             {C D}
+             (a : option (A * B * D))
+             (k : A -> B -> D -> option (C * B * D))
+    : option (C * B * D) :=
+    Ifopt a as a_opt Then
+      match a_opt with (a, bin', env') => k a bin' env' end
+      Else None.
+
+  Definition DecodeBindOpt
+             {C}
+             (a : option (A * B))
+             (k : A -> B -> option (C * B))
+    : option (C * B) :=
+    Ifopt a as a_opt Then
+      match a_opt with (a, bin') => k a bin' end
+    Else None.
+
 End Specifications.
+
+Notation "`( a , b , env ) <- c ; k" :=
+  (DecodeBindOpt2 c%binencoders (fun a b env => k%binencoders)) : binencoders_scope.
+
+Notation "`( a , b ) <- c ; k" :=
+  (DecodeBindOpt c%binencoders (fun a b => k%binencoders)) : binencoders_scope.
+
+Open Scope binencoders_scope.
+Global Unset Implicit Arguments.
