src/BinEncoders/Env/Lib2/AsciiOpt.v
@@ -1,0 +1,52 @@
+Require Import
+        Fiat.BinEncoders.Env.Common.Specs
+        Fiat.BinEncoders.Env.Lib2.WordOpt.
+Require Import
+        Bedrock.Word
+        Coq.Strings.Ascii
+        Coq.Numbers.BinNums
+        Coq.NArith.BinNat.
+
+Section Ascii.
+  Context {B : Type}.
+  Context {cache : Cache}.
+  Context {cacheAddNat : CacheAdd cache nat}.
+  Context {transformer : Transformer B}.
+  Context {transformerUnit : TransformerUnitOpt transformer bool}.
+
+  Definition encode_ascii (c : ascii) (ce : CacheEncode) : B * CacheEncode :=
+    encode_word (NToWord 8 (N_of_ascii c)) ce.
+
+  Definition decode_ascii (b : B) (cd : CacheDecode) : option (ascii * B * CacheDecode) :=
+    `(n, b, cd) <- decode_word (sz:=8) b cd;
+      Some (ascii_of_N (wordToN n), b, cd).
+
+  Open Local Scope nat.
+  Theorem Ascii_decode_correct :
+    encode_decode_correct_f cache transformer (fun n => True) encode_ascii decode_ascii.
+  Proof.
+    unfold encode_decode_correct, encode_ascii, decode_ascii.
+    intros env env' xenv c c' ext Eeq Ppred Penc.
+    destruct (Word_decode_correct _ _ _ _ _ ext Eeq I Penc) as [? [? ?] ].
+    rewrite H; simpl.
+    eexists; intuition eauto.
+    repeat f_equal.
+    rewrite wordToN_nat. rewrite NToWord_nat.
+    destruct (wordToNat_natToWord' 8 (BinNat.N.to_nat (N_of_ascii c))).
+    assert (x0 = 0).
+    { destruct x0; eauto; exfalso.
+      remember (wordToNat (natToWord 8 (BinNat.N.to_nat (N_of_ascii c)))) as xx; clear Heqxx.
+      replace (xx + S x0 * pow2 8) with (256 + (xx + x0 * 256)) in H1.
+      assert (BinNat.N.to_nat (N_of_ascii c) < 256).
+      assert (N.lt (N_of_ascii c) 256).
+      clear H. induction c; repeat (match goal with
+                                    | B : bool |- _ => destruct B
+                                    end); simpl; unfold Nlt; eauto.
+      change (256%nat) with (N.to_nat 256).
+      apply Nomega.Nlt_out. eauto.
+      omega. change (pow2 8) with 256. omega.
+    }
+    subst. rewrite <- plus_n_O in H1. rewrite H1. clear H1.
+    rewrite Nnat.N2Nat.id. rewrite ascii_N_embedding. eauto.
+  Qed.
+End Ascii.
