src/BinEncoders/Env/Lib2/NatOpt.v
@@ -1,0 +1,43 @@
+Require Import
+        Fiat.BinEncoders.Env.Common.Specs
+        Fiat.BinEncoders.Env.Lib2.WordOpt.
+Require Import
+        Bedrock.Word.
+
+Section Nat.
+  Variable sz : nat.
+
+  Context {B : Type}.
+  Context {cache : Cache}.
+  Context {cacheAddNat : CacheAdd cache nat}.
+  Context {transformer : Transformer B}.
+  Context {transformerUnit : TransformerUnitOpt transformer bool}.
+
+  Definition encode_nat (n : nat) (ce : CacheEncode) : B * CacheEncode :=
+    encode_word (natToWord sz n) ce.
+
+  Definition decode_nat (b : B) (cd : CacheDecode) : option (nat * B * CacheDecode) :=
+    `(w, b, cd) <- decode_word (sz:=sz) b cd;
+      Some (wordToNat w, b, cd).
+
+  Local Open Scope nat.
+  Theorem Nat_decode_correct :
+    encode_decode_correct_f cache transformer (fun n => n < pow2 sz) encode_nat decode_nat.
+  Proof.
+    unfold encode_decode_correct_f, encode_nat, decode_nat.
+    intros env xenv xenv' n n' ext Eeq Ppred Penc.
+    destruct (Word_decode_correct _ _ _ _ _ ext Eeq I Penc) as [? [? ?] ].
+    - rewrite H; simpl; eexists; intuition eauto.
+      repeat f_equal.
+      destruct (wordToNat_natToWord' sz n).
+      assert (x0 = 0).
+      { destruct x0; eauto.
+        rewrite <- H1 in Ppred. exfalso. simpl in Ppred.
+        clear - Ppred.
+        replace (wordToNat (natToWord sz n) + (pow2 sz + x0 * pow2 sz)) with
+        (pow2 sz + (wordToNat (natToWord sz n) + x0 * pow2 sz)) in Ppred by omega.
+        remember (wordToNat (natToWord sz n) + x0 * pow2 sz) as n'; clear Heqn'.
+        omega. }
+      rewrite H2 in H1. simpl in H1. rewrite <- plus_n_O in H1. eauto.
+  Qed.
+End Nat.
