src/BinEncoders/Env/Lib2/SteppingListOpt.v
@@ -1,0 +1,180 @@
+Require Import
+        Fiat.BinEncoders.Env.Common.Specs
+        Fiat.BinEncoders.Env.Lib2.FixListOpt.
+Require Export
+        Coq.Lists.List.
+
+Section SteppingList.
+  Context {A : Type}. (* data type *)
+  Context {B : Type}. (* bin type *)
+  Context {P : Type}. (* cache pointer type *)
+  Context {cache : Cache}.
+  Context {transformer : Transformer B}.
+
+  Variable fuel : nat.
+  Variable A_halt : A.
+  Variable A_halt_dec : forall a, {a = A_halt} + {~ a = A_halt}.
+  Variable A_predicate : A -> Prop.
+  Variable A_encode : A -> CacheEncode -> B * CacheEncode.
+  Variable A_decode : B -> CacheDecode -> option (A * B * CacheDecode).
+  Variable A_decode_pf : encode_decode_correct_f cache transformer A_predicate A_encode A_decode.
+
+  Variable P_predicate : P -> Prop.
+  Variable P_predicate_dec : forall p, {P_predicate p} + {~ P_predicate p}.
+  Variable P_encode : P -> CacheEncode -> B * CacheEncode.
+  Variable P_decode : B -> CacheDecode -> option (P * B * CacheDecode).
+  Variable P_decode_pf : encode_decode_correct_f cache transformer P_predicate P_encode P_decode.
+
+  Variable X_encode : bool -> CacheEncode -> B * CacheEncode.
+  Variable X_decode : B -> CacheDecode -> option (bool * B * CacheDecode).
+  Variable X_decode_pf : encode_decode_correct_f cache transformer (fun _ => True) X_encode X_decode.
+
+  Variable cacheAdd : CacheAdd cache (list A * P).
+  Variable cacheGet : CacheGet cache (list A) P.
+  Variable cachePeek : CachePeek cache P.
+
+  Fixpoint encode_list_step (l : list A) (ce : CacheEncode) : B * CacheEncode :=
+    match l with
+    | nil => let (b1, e1) := X_encode false ce in
+             let (b2, e2) := A_encode A_halt e1 in
+                 (transform b1 b2, e2)
+    | cons x l' =>
+      match getE ce l with
+      | Some position =>
+        if P_predicate_dec position
+        then let (b1, e1) := X_encode true ce in
+             let (b2, e2) := P_encode position e1 in
+                 (transform b1 b2, e2)
+        else let (b1, e1) := X_encode false ce in
+             let (b2, e2) := A_encode x e1 in
+             let (b3, e3) := encode_list_step l' e2 in
+                 (transform (transform b1 b2) b3, addE e3 (l, peekE ce))
+      | None => let (b1, e1) := X_encode false ce in
+                let (b2, e2) := A_encode x e1 in
+                let (b3, e3) := encode_list_step l' e2 in
+                    (transform (transform b1 b2) b3, addE e3 (l, peekE ce))
+      end
+    end.
+
+  Fixpoint decode'_list_step (f : nat) (b : B) (cd : CacheDecode) : option (list A * B * CacheDecode) :=
+    `(br, b1, e1) <- X_decode b cd;
+      If br Then
+       `(ps, b2, e2) <- P_decode b1 e1;
+        match getD cd ps with
+        | Some l => Some (l, b2, e2)
+        | None => None (* bogus *)
+        end
+      Else
+        (`(a , b2, e2) <- A_decode b1 e1;
+           If A_halt_dec a Then
+              Some (nil, b2, e2)
+              Else
+              match f with
+              | O => None (* bogus *)
+              | S f' => `(l, b3, e3) <- decode'_list_step f' b2 e2;
+                          Some (a :: l, b3, addD e3 (a :: l, peekD cd))
+              end).
+
+  Definition decode_list_step := decode'_list_step fuel.
+
+  Theorem SteppingList_decode_correct :
+    encode_decode_correct_f
+      cache transformer
+      (fun ls => A_predicate A_halt /\ |ls| <= fuel /\ (forall x, In x ls -> A_predicate x /\
+                                                                             ~ x = A_halt))
+      encode_list_step decode_list_step.
+  Proof.
+    unfold encode_decode_correct_f.
+    intros env xenv xenv' l l' ext Eeq [Ppredh [PPredlen PPredA]] Penc;
+      subst.
+    unfold decode_list_step in *; simpl in *.
+    generalize dependent l'; generalize dependent fuel; clear fuel;
+      generalize dependent env; 
+      generalize dependent xenv; 
+      generalize ext; generalize dependent xenv';
+    induction l; intros; simpl in *.
+    { destruct (X_encode false env) eqn: ?.
+      destruct (A_encode A_halt c) eqn: ?.
+      inversion Penc; subst; clear Penc.
+      destruct (X_decode_pf _ _ _ _ _ (transform b0 ext0) Eeq I Heqp) as [? [? ?]]; subst.
+      rewrite <- transform_assoc.
+      destruct fuel eqn: ?; subst; simpl in *.
+      { rewrite H; simpl.
+        destruct (A_decode_pf _ _ _ _ _ ext0 H0 Ppredh Heqp0) as [? [? ?]]; subst.
+        rewrite H1.
+        simpl.
+        destruct (A_halt_dec A_halt); simpl; eexists; eauto.
+        congruence.
+      }
+      { rewrite H; simpl.
+        destruct (A_decode_pf _ _ _ _ _ ext0 H0 Ppredh Heqp0) as [? [? ?]]; subst.
+        rewrite H1.
+        simpl.
+        destruct (A_halt_dec A_halt); simpl; eexists; eauto.
+        congruence.
+      } 
+    }
+    destruct fuel; try omega; simpl.
+    destruct (getE env (a :: l)) eqn: ?.
+    - destruct (P_predicate_dec p).
+      + destruct (X_encode true env) eqn: ? ;
+          destruct (P_encode p c) eqn: ?; intros; injections.
+        destruct (X_decode_pf _ _ _ _ _ (transform b0 ext0) Eeq I Heqp1) as [? [? ?]]; subst.
+        rewrite <- transform_assoc; rewrite H; simpl.
+        destruct (P_decode_pf _ _ _ _ _ ext0 H0 p0 Heqp0) as [? [? ?]];
+          subst; rewrite H1; simpl.
+        eapply get_correct in Heqo; eauto; rewrite Heqo.
+        eauto.
+      + destruct (X_encode false env) eqn: ? ;
+          destruct (P_encode p c) eqn: ?; intros; injections.
+        destruct (A_encode a c) eqn: ?.
+        destruct (encode_list_step l c1) eqn: ?.
+        injections.
+        destruct (X_decode_pf _ _ _ _ _ (transform b1 (transform b2 ext0))
+                              Eeq I Heqp0) as [? [? ?]]; subst.
+        rewrite <- !transform_assoc; rewrite H; simpl.
+        destruct (A_decode_pf _ _ _ _ _ (transform b2 ext0) H0 (proj1 (PPredA _ (or_introl _ eq_refl))) Heqp2) as [? [? ?]]; subst.
+        rewrite H1; simpl.
+        destruct (A_halt_dec a); simpl.
+        elimtype False; apply (proj2 (PPredA _ (or_introl _ eq_refl)));
+          eauto.
+        eapply (fun H => IHl H _ ext0) in Heqp3; intros.
+        destruct_ex; intuition.
+        rewrite H4; simpl.
+        eexists; intuition eauto.
+        erewrite peek_correct.
+        eapply add_correct.
+        eauto.
+        eauto.
+        eapply PPredA; eauto.
+        eauto.
+        omega.
+    - destruct (X_encode false env) eqn: ? ;
+        destruct (A_encode a c) eqn: ?.
+      destruct (encode_list_step l c0) eqn: ?.
+      injections.
+      destruct (X_decode_pf _ _ _ _ _ (transform b0 (transform b1 ext0))
+                            Eeq I Heqp) as [? [? ?]]; subst.
+      rewrite <- !transform_assoc; rewrite H; simpl.
+      destruct (A_decode_pf _ _ _ _ _ (transform b1 ext0) H0 (proj1 (PPredA _ (or_introl _ eq_refl))) Heqp0) as [? [? ?]]; subst.
+      rewrite H1; simpl.
+      destruct (A_halt_dec a); simpl.
+      elimtype False; apply (proj2 (PPredA _ (or_introl _ eq_refl)));
+        eauto.
+      eapply (fun H => IHl H _ ext0) in Heqp1; intros.
+      destruct_ex; intuition.
+      rewrite H4; simpl.
+      eexists; intuition eauto.
+      erewrite peek_correct.
+      eapply add_correct.
+      eauto.
+      eauto.
+      eapply PPredA; eauto.
+      eauto.
+      omega.
+      Grab Existential Variables.
+      eauto.
+      eauto.
+  Qed.
+End SteppingList.
+
