src/BinEncoders/Env/Lib2/StringOpt.v
@@ -1,0 +1,61 @@
+Require Import
+        Fiat.BinEncoders.Env.Common.Specs
+        Fiat.BinEncoders.Env.Lib2.AsciiOpt.
+Require Import
+        Bedrock.Word
+        Coq.Strings.Ascii
+        Coq.Strings.String.
+
+Section String.
+  (* this has an exact idential structure to _FixList_ *)
+  Context {A : Type}.
+  Context {B : Type}.
+  Context {cache : Cache}.
+  Context {cacheAddNat : CacheAdd cache nat}.
+  Context {transformer : Transformer B}.
+  Context {transformerUnit : TransformerUnitOpt transformer bool}.
+
+  Fixpoint encode_string (xs : string) (ce : CacheEncode) : B * CacheEncode :=
+    match xs with
+    | EmptyString => (transform_id, ce)
+    | String x xs' => let (b1, env1) := encode_ascii x ce in
+                      let (b2, env2) := encode_string xs' env1 in
+                          (transform b1 b2, env2)
+    end.
+
+  Fixpoint decode_string (s : nat) (b : B) (cd : CacheDecode) : option (string * B * CacheDecode) :=
+    match s with
+    | O => Some (EmptyString, b, cd)
+    | S s' => `(x, b1, e1) <- decode_ascii b cd;
+              `(xs, b2, e2) <- decode_string s' b1 e1;
+              Some (String x xs, b2, e2)
+    end.
+
+  Local Opaque encode_ascii.
+  Theorem String_decode_correct :
+    forall sz,
+      encode_decode_correct_f
+        cache transformer
+        (fun ls => length ls = sz)
+        encode_string (decode_string sz).
+  Proof.
+    intros ? env env' xenv l l' ext Eeq Ppred Penc.
+    subst.
+    generalize dependent env.
+    revert env' xenv l'.
+    induction l.
+    { intros.
+      inversion Penc; subst; clear Penc.
+      rewrite transform_id_left; eexists; intuition eauto.  }
+    { intros.
+      simpl in *.
+      destruct (encode_ascii a env) eqn: ?.
+      destruct (encode_string l c) eqn: ?.
+      injection Penc; intros; subst.
+      destruct (Ascii_decode_correct _ _ _ _ _ (transform b0 ext) Eeq I Heqp) as [? [? ?] ].
+      rewrite <- transform_assoc, H; simpl.
+      destruct (IHl _ _ _ _ H0 Heqp0) as [? [? ?] ].
+      rewrite H1; simpl; eexists; eauto.
+    }
+  Qed.
+End String.
