src/BinEncoders/Env/Lib2/SumTypeOpt.v
@@ -1,0 +1,132 @@
+Require Import
+        Fiat.Common.ilist
+        Fiat.Common.SumType
+        Fiat.Examples.DnsServer.Packet
+        Fiat.BinEncoders.Env.Common.Specs.
+
+Require Import
+        Coq.Sets.Ensembles
+        Bedrock.Word.
+
+Section SumType.
+
+  Context {B : Type}.
+  Context {cache : Cache}.
+  Context {cacheAddNat : CacheAdd cache nat}.
+  Context {transformer : Transformer B}.
+  Context {transformerUnit : TransformerUnitOpt transformer bool}.
+
+  Definition encode_SumType {m}
+             (types : Vector.t Type m)
+             (encoders : ilist (B := fun T => T -> CacheEncode -> B * CacheEncode) types)
+             (st : SumType types)
+    : CacheEncode -> B * CacheEncode :=
+    ith encoders (SumType_index types st) (SumType_proj types st).
+
+  Definition decode_SumType {m}
+             (types : Vector.t Type m)
+             (decoders : ilist (B := fun T => B -> CacheDecode -> option (T * B * CacheDecode)) types)
+             (idx : Fin.t m)
+             (b : B)
+             (cd : CacheDecode)
+    : option (SumType types * B * CacheDecode) :=
+    `(a, b', cd') <- ith decoders idx b cd;
+      Some (inj_SumType types idx a, b', cd').
+
+  Lemma tri_proj_eq {A C D} : forall a c d (acd : A * C * D),
+      a = fst (fst acd)
+      -> c = snd (fst acd)
+      -> d = snd acd
+      -> acd = ((a, c), d).
+  Proof.
+    intros; subst; intuition.
+  Qed.
+
+  Theorem SumType_decode_correct {m}
+          (types : Vector.t Type m)
+          (encoders : ilist (B := fun T => T -> CacheEncode -> B * CacheEncode) types)
+          (decoders : ilist (B := fun T => B -> CacheDecode -> option (T * B * CacheDecode)) types)
+          (invariants : forall idx, Vector.nth types idx -> Prop)
+          (encoders_decoders_correct : forall idx,
+              encode_decode_correct_f
+                cache transformer
+                (fun st => invariants idx st)
+                (ith encoders idx)
+                (ith decoders idx))
+          idx
+    :
+    encode_decode_correct_f cache transformer (fun st => SumType_index types st = idx /\ invariants _ (SumType_proj types st))
+                          (encode_SumType types encoders)
+                          (decode_SumType types decoders idx).
+  Proof.
+    revert types encoders decoders invariants encoders_decoders_correct.
+    unfold encode_decode_correct_f, encode_SumType, decode_SumType.
+    induction types.
+    - inversion idx.
+    - revert types IHtypes h; pattern n, idx; apply Fin.caseS;
+        clear n idx; intros; destruct H0.
+      + (* First element *)
+        destruct types.
+        * unfold SumType in data; simpl in *.
+          destruct (encoders_decoders_correct Fin.F1 _ _ _ _ _ ext H H2 H1) as [? [? ?] ]; simpl in *.
+          rewrite H3; simpl; eexists; eauto.
+        * destruct data; try discriminate; simpl in *.
+          destruct (encoders_decoders_correct Fin.F1 _ _ _ _ _ ext H H2 H1) as [? [? ?] ]; simpl in *.
+          match goal with
+            |- context [@prim_fst ?A ?B ?a ?z ?k] =>
+            replace (@prim_fst A B a z k) with (Some (h1, ext, x))
+              by (rewrite <- H3; reflexivity)
+          end.
+          simpl; eauto.
+      + (* Second element *)
+        destruct types; try discriminate.
+        destruct data; try discriminate.
+        assert (p = SumType_index (Vector.cons Type h0 n types) s) by
+            (apply Fin.FS_inj in H0;
+             rewrite <- H0; reflexivity).
+        assert (invariants
+                  (Fin.FS (SumType_index (Vector.cons Type h0 n types) s))
+                  (SumType_proj (Vector.cons Type h0 n types) s)) as H3' by
+            eapply H2.
+        assert (ith encoders
+                    (Fin.FS (SumType_index (Vector.cons Type h0 n types) s))
+                    (SumType_proj (Vector.cons Type h0 n types) s) env =
+                (bin, xenv)) as H1' by apply H1; clear H1.
+        assert (exists xenv' : CacheDecode,
+     (`(a, b', cd') <- ith (ilist_tl decoders) p (transform bin ext) env';
+      Some
+        (inj_SumType (Vector.cons Type h0 n types) p a, b',
+        cd')) = Some (s, ext, xenv') /\ Equiv xenv xenv').
+        { eapply (IHtypes p (ilist_tl encoders) (ilist_tl decoders)
+                 (fun idx => invariants (Fin.FS idx))); eauto.
+          intros.
+          destruct (encoders_decoders_correct (Fin.FS _) _ _ _ _ _ ext0 H1 H4 H5) as [? [? ?] ]; simpl in *.
+          eexists; intuition eauto.
+        }
+        destruct_ex; intuition.
+        eexists; split; eauto.
+        match goal with
+            |- context [ith ?d ?idx ?tb ?env'] =>
+            destruct (ith d idx tb env') eqn: ?
+          end.
+        simpl in Heqo.
+        unfold ilist_tl in H4.
+        match type of H4 with
+          context [@ith ?A ?B ?m ?As ?il ?n ?il' ?M] =>
+          assert (@ith A B m As il n il' M = Some p0) as Heqo'
+              by (simpl; apply Heqo);
+            rewrite Heqo' in H4
+        end.
+        destruct p0 as [ [? ?] ?]; simpl in *.
+        injection H4; intros.
+        repeat f_equal; eauto.
+        match type of H4 with
+          context [@ith ?A ?B ?m ?As ?il ?n ?il' ?M] =>
+          assert (@ith A B m As il n il' M = None) as Heqo'
+              by (simpl; apply Heqo);
+            rewrite Heqo' in H4; discriminate
+        end.
+  Qed.
+End SumType.
+
+Arguments SumType : simpl never.
