src/BinEncoders/Env/Lib2/WordOpt.v
@@ -1,0 +1,58 @@
+Require Import
+        Fiat.Common
+        Fiat.Computation.Notations
+        Fiat.BinEncoders.Env.Common.Specs.
+
+Require Import
+        Bedrock.Word.
+
+Unset Implicit Arguments.
+Section Word.
+  Context {sz : nat}.
+
+  Context {B : Type}.
+  Context {cache : Cache}.
+  Context {cacheAddNat : CacheAdd cache nat}.
+  Context {transformer : Transformer B}.
+  Context {transformerUnit : TransformerUnitOpt transformer bool}.
+
+  Fixpoint encode_word' (s : nat) (w : word s) : B :=
+    match w with
+    | WO => transform_id
+    | WS b s' w' => transform_push_opt b (@encode_word' s' w')
+    end.
+
+  Definition encode_word (w : word sz) (ce : CacheEncode) : B * CacheEncode :=
+    (encode_word' sz w, addE ce sz).
+
+  Fixpoint decode_word' (s : nat) (b : B) : option (word s * B) :=
+    match s with
+    | O => Some (WO, b)
+    | S s' =>
+      `(c, b') <- transform_pop_opt b;
+      `(w, bx) <- decode_word' s' b';
+       Some (WS c w, bx)
+    end.
+
+  Definition decode_word (b : B) (cd : CacheDecode) : option (word sz * B * CacheDecode) :=
+    Ifopt decode_word' sz b as decoded Then Some (decoded, addD cd sz) Else None.
+
+  Theorem Word_decode_correct :
+    encode_decode_correct_f cache transformer (fun _ => True) encode_word decode_word.
+  Proof.
+    unfold encode_decode_correct, encode_word, decode_word.
+    intros env env' xenv w w' ext Eeq _ Penc.
+    inversion Penc; subst; clear Penc.
+    generalize dependent sz.
+    induction w; simpl in *.
+    { eexists; split; eauto; try rewrite !transform_id_left; 
+      eauto using add_correct. }
+    { rewrite transform_push_step_opt.
+      rewrite transform_push_pop_opt.
+      destruct_ex; intuition.
+      destruct (decode_word' n (transform (encode_word' n w) ext)) as [ [? ?] | ] eqn: ?; simpl in *; try discriminate.
+      injections; eexists; split; eauto using add_correct.
+      rewrite Heqo; simpl; f_equal.
+    }
+  Qed.
+End Word.
