src/Computation/Notations.v
@@ -4,4 +4,16 @@ Reserved Notation "x ;; z" (at level 42, right associativity).*)
 Reserved Infix "↝" (at level 70).
 Reserved Notation "⟦ x 'in' xs | P ⟧" (at level 70).
 
+Reserved Notation "x <- y ; z"
+         (at level 81, right associativity,
+          format "'[v' x  <-  y ; '/' z ']'").
+
+Reserved Notation "`( a , b ) <- c ; k"
+         (at level 81, right associativity,
+          format "'[v' `( a ,  b )  <-  c ; '/' k ']'").
+
+Reserved Notation "`( a , b , c ) <- d ; k"
+         (at level 81, right associativity,
+          format "'[v' `( a ,  b ,  c )  <-  d ; '/' k ']'").
+
 Delimit Scope comp_scope with comp.
